src/program_proof/grove_shared/urpc_spec.v
@@ -12,58 +12,74 @@ Context `{!urpcregG Σ}.
 Context `{HPRE: !gooseGlobalGS Σ}.
 
 (* Higher-level interface for defining a uRPC spec. *)
-Record RpcSpec {spec_ty : Type} : Type :=
-  Build_uRPCSpec {
+Record RpcSpec :=
+  {
+    spec_ty : Type;
     spec_Pre : spec_ty → list u8 → iProp Σ;
-    spec_Post : spec_ty → list u8 → list u8 → iProp Σ }.
+    spec_Post : spec_ty → list u8 → list u8 → iProp Σ
+  }.
 
-Program Definition uRPCSpec_Spec {spec_ty:Type} (spec : RpcSpec (spec_ty:=spec_ty)) : savedSpecO Σ (list u8) (list u8) :=
+Program Definition RpcSpec_Spec (spec : RpcSpec) : savedSpecO Σ (list u8) (list u8) :=
   λ args, λne (Φ : list u8 -d> iPropO Σ), (∃ x,
     spec.(spec_Pre) x args ∗ (∀ rep, spec.(spec_Post) x args rep -∗ Φ rep))%I.
 Next Obligation. solve_proper. Qed.
 
-Definition is_urpc_spec Γsrv (host:u64) (rpcid:u64) {spec_ty:Type} (spec : uRPCSpec (spec_ty:=spec_ty)) :=
-  is_urpc_spec_pred Γsrv host rpcid (uRPCSpec_Spec spec).
+Definition is_urpc_spec Γsrv (host:u64) (rpcid:u64) (spec : RpcSpec) :=
+  is_urpc_spec_pred Γsrv host rpcid (RpcSpec_Spec spec).
 
-Fixpoint dom_uRPCSpecList (l: list (u64 * uRPCSpec_Spec)) : gset u64 :=
+Local Example spec_iprop :=
+  {|
+  spec_ty := iProp Σ;
+  spec_Pre := λ (_:iProp Σ) _, True%I;
+  spec_Post := λ _ _ _, True%I
+  |}.
+
+(* XXX: using this because [list] is not universe polymorphic. *)
+Polymorphic Cumulative Inductive plist (A : Type) :=
+| pnil : plist A
+| pcons : A -> plist A -> plist A.
+Arguments pnil {A}.
+Arguments pcons {A} a l.
+(* FIXME: notation for this? *)
+
+Fixpoint dom_RpcSpec_list (l: plist (u64 * RpcSpec)) : gset u64 :=
   match l with
-  | spec_nil => ∅
-  | spec_cons x l => {[ spec_rpcid x ]} ∪ dom_uRPCSpecList l
+  | pnil => ∅
+  | pcons x l => {[ x.1 ]} ∪ dom_RpcSpec_list l
   end.
 
-Fixpoint handler_uRPCSpecList γ host (l : uRPCSpecList) :=
+Fixpoint is_urpc_spec_list γ host (l : plist (u64 * RpcSpec)) :=
   match l with
-  | spec_nil => True%I
-  | spec_cons x l =>
-    (is_urpc_spec γ host x ∗
-                handler_uRPCSpecList γ host l)%I
+  | pnil => True%I
+  | pcons x l =>
+    (is_urpc_spec γ host x.1 x.2 ∗ is_urpc_spec_list γ host l)%I
   end.
 
-Fixpoint uRPCSpecList_wf (l : uRPCSpecList) : Prop :=
+Fixpoint RpcSpec_list_wf (l : plist (u64 * RpcSpec)) : Prop :=
   match l with
-  | spec_nil => True
-  | spec_cons x l =>
-    (spec_rpcid x ∉ dom_uRPCSpecList l) ∧ uRPCSpecList_wf l
+  | pnil => True
+  | pcons x l =>
+    (x.1 ∉ dom_RpcSpec_list l) ∧ RpcSpec_list_wf l
   end.
 
-Lemma handler_is_init_list (host : chan) (specs: uRPCSpecList) (Hwf: uRPCSpecList_wf specs) :
+Lemma alloc_is_urpc_list (host : chan) (specs: plist (u64 * RpcSpec)) (Hwf: RpcSpec_list_wf specs) :
    host c↦ ∅ ={⊤}=∗ ∃ γ,
-   is_urpc_dom γ (dom_uRPCSpecList specs) ∗
-   handler_uRPCSpecList γ host specs.
+   is_urpc_dom γ (dom_RpcSpec_list specs) ∗
+   is_urpc_spec_list γ host specs.
 Proof.
   iIntros "Hchan".
   iMod (map_init (∅ : gmap u64 gname)) as (γmap) "Hmap_ctx".
-  iMod (own_alloc (to_agree (dom_uRPCSpecList specs : gsetO u64))) as (γdom) "#Hdom".
+  iMod (own_alloc (to_agree (dom_RpcSpec_list specs : gsetO u64))) as (γdom) "#Hdom".
   { econstructor. }
   set (Γsrv := {| scmap_name := γmap; scset_name := γdom |}).
   iMod (inv_alloc urpc_serverN _ ((server_chan_inner host Γsrv)) with "[Hchan]") as "#Hinv".
   { iNext. iExists _. iFrame.
     rewrite big_sepS_empty //. }
   iExists Γsrv.
-  iAssert (∀ specs', ⌜ uRPCSpecList_wf specs' ⌝ ∗ ⌜ dom_uRPCSpecList specs' ⊆  dom_uRPCSpecList specs ⌝ →
-           |==> ∃ gnames : gmap u64 gname, ⌜ dom gnames = dom_uRPCSpecList specs' ⌝ ∗
+  iAssert (∀ specs', ⌜ RpcSpec_list_wf specs' ⌝ ∗ ⌜ dom_RpcSpec_list specs' ⊆  dom_RpcSpec_list specs ⌝ →
+           |==> ∃ gnames : gmap u64 gname, ⌜ dom gnames = dom_RpcSpec_list specs' ⌝ ∗
            map_ctx (scmap_name Γsrv) 1 gnames ∗
-           handler_uRPCSpecList Γsrv host specs')%I with "[Hmap_ctx]" as "H"; last first.
+           is_urpc_spec_list Γsrv host specs')%I with "[Hmap_ctx]" as "H"; last first.
   { iMod ("H" with "[]") as (?) "(_&_&$)"; eauto. }
   iIntros (specs').
   iInduction specs' as [| hd spec] "IH".
@@ -74,70 +90,7 @@ Proof.
     { iPureIntro. split.
       - destruct Hwf' as (_&?); eauto.
       - etransitivity; last eassumption. set_solver. }
-    iMod (saved_spec_alloc (uRPCSpec_Spec hd)) as (γsave) "#Hsaved".
-    iMod (map_alloc_ro (spec_rpcid hd) γsave
-            with "Hmap_ctx") as "(Hmap_ctx&#Hsaved_name)"; auto.
-    { apply not_elem_of_dom. destruct (Hwf') as (?&?). rewrite Hdom. eauto. }
-    iExists _; iFrame. iModIntro.
-    iSplit.
-    { iPureIntro. rewrite ?dom_insert_L Hdom. set_solver. }
-    iExists _, _. iFrame "#".
-    { iPureIntro. simpl in Hdom'. set_solver. }
-  }
-Qed.
-
-
-(* More general version of above initialization lemma *)
-Implicit Type (l:list (u64 * savedSpecO Σ (list u8) (list u8))).
-Fixpoint is_urpc_spec_pred_list γ host l :=
-  match l with
-  | [] => True%I
-  | x :: l =>
-    (is_urpc_spec_pred γ host x.1 x.2 ∗ is_urpc_spec_pred_list γ host l)%I
-  end.
-
-Fixpoint dom_spec_list l : gset u64 :=
-  match l with
-  | [] => ∅
-  | x :: l => {[ x.1 ]} ∪ dom_spec_list l
-  end.
-
-Fixpoint spec_list_wf l : Prop :=
-  match l with
-  | [] => True
-  | x :: l =>
-    (x.1 ∉ dom_spec_list l) ∧ spec_list_wf l
-  end.
-
-Lemma handler_is_init_list2 (host : chan) specs (Hwf: spec_list_wf specs) :
-   host c↦ ∅ ={⊤}=∗ ∃ γ,
-   is_urpc_dom γ (dom_spec_list specs) ∗
-   is_urpc_spec_pred_list γ host specs.
-Proof.
-  iIntros "Hchan".
-  iMod (map_init (∅ : gmap u64 gname)) as (γmap) "Hmap_ctx".
-  iMod (own_alloc (to_agree (dom_spec_list specs : gsetO u64))) as (γdom) "#Hdom".
-  { econstructor. }
-  set (Γsrv := {| scmap_name := γmap; scset_name := γdom |}).
-  iMod (inv_alloc urpc_serverN _ ((server_chan_inner host Γsrv)) with "[Hchan]") as "#Hinv".
-  { iNext. iExists _. iFrame.
-    rewrite big_sepS_empty //. }
-  iExists Γsrv.
-  iAssert (∀ specs', ⌜ spec_list_wf specs' ⌝ ∗ ⌜ dom_spec_list specs' ⊆  dom_spec_list specs ⌝ →
-           |==> ∃ gnames : gmap u64 gname, ⌜ dom gnames = dom_spec_list specs' ⌝ ∗
-           map_ctx (scmap_name Γsrv) 1 gnames ∗
-           is_urpc_spec_pred_list Γsrv host specs')%I with "[Hmap_ctx]" as "H"; last first.
-  { iMod ("H" with "[]") as (?) "(_&_&$)"; eauto. }
-  iIntros (specs').
-  iInduction specs' as [| hd spec] "IH".
-  { iIntros (?). iModIntro. iExists ∅. iFrame.
-    rewrite ?dom_empty_L //. }
-  { iIntros ((Hwf'&Hdom')).
-    iMod ("IH" with "[$] []") as (gnames Hdom) "(Hmap_ctx&Hmap)".
-    { iPureIntro. split.
-      - destruct Hwf' as (_&?); eauto.
-      - etransitivity; last eassumption. set_solver. }
-    iMod (saved_spec_alloc hd.2) as (γsave) "#Hsaved".
+    iMod (saved_spec_alloc (RpcSpec_Spec hd.2)) as (γsave) "#Hsaved".
     iMod (map_alloc_ro (hd.1) γsave
             with "Hmap_ctx") as "(Hmap_ctx&#Hsaved_name)"; auto.
     { apply not_elem_of_dom. destruct (Hwf') as (?&?). rewrite Hdom. eauto. }
@@ -154,47 +107,44 @@ End rpc_global_defs.
 Section urpc_spec_impl.
 Context `{!heapGS Σ, !urpcregG Σ}.
 
-Definition is_urpc_handler (f : val) (spec : uRPCSpec)
+Definition is_urpc_handler (f : val) (spec : RpcSpec)
    : iProp Σ :=
-  ∀ (x : spec.(spec_ty)) (reqData : list u8) req repptr dummy_rep_sl dummy,
+  ∀ (x : spec.(spec_ty)) (reqData : list u8) req rep,
   {{{
     own_slice_small req byteT 1 reqData ∗
-    repptr ↦[slice.T byteT] (slice_val dummy_rep_sl) ∗
-    own_slice (V:=u8) dummy_rep_sl byteT 1 dummy ∗
+    rep ↦[slice.T byteT] (slice_val Slice.nil) ∗
     spec.(spec_Pre) x reqData
   }}}
-    f (slice_val req) #repptr
+    f (slice_val req) #rep
   {{{ rep_sl q repData, RET #();
-      repptr ↦[slice.T byteT] (slice_val rep_sl) ∗
+      rep ↦[slice.T byteT] (slice_val rep_sl) ∗
       own_slice_small rep_sl byteT q repData ∗
       spec.(spec_Post) x reqData repData
   }}}.
 
-(** Lift handler registration and RPC calls to uRPCSpec *)
+(** Lift handler registration and RPC calls to RpcSpec *)
 
 Lemma urpc_handler_to_handler f spec :
   is_urpc_handler f spec -∗
-  is_urpc_handler_pred f (uRPCSpec_Spec spec).
+  is_urpc_handler_pred f (RpcSpec_Spec spec).
 Proof.
   rewrite /is_urpc_handler_pred.
   iIntros "#Hf %reqData %Cont %req %repptr !# %Φ Hpre HΦ".
   iDestruct "Hpre" as "(Hreq & Hrepptr & Hpre)". iSimpl in "Hpre".
   iDestruct "Hpre" as (x) "[Hpre Hcont]".
   wp_apply ("Hf" with "[$Hrepptr $Hpre $Hreq]").
-  { iApply own_slice_zero. }
   iIntros (???) "(Hrepptr & Hrep & Hpost)".
   iApply "HΦ". iFrame. iApply "Hcont". done.
 Qed.
 
-Lemma wp_Client__Call_uRPCSpec γsmap (cl_ptr:loc) (rpcid:u64) (host:u64) req rep_out_ptr
-      (timeout_ms : u64) dummy_sl_val (reqData:list u8) (spec : uRPCSpec) (x : spec.(spec_ty)) :
-  rpcid = spec.(spec_rpcid) →
-  is_urpc_spec γsmap host spec -∗
+Lemma wp_Client__Call γsmap (cl_ptr:loc) (rpcid:u64) (host:u64) req rep_out_ptr
+      (timeout_ms : u64) dummy_sl_val (reqData:list u8) (spec : RpcSpec) (x : spec.(spec_ty)) :
   {{{
-      own_slice_small req byteT 1 reqData ∗
-      rep_out_ptr ↦[slice.T byteT] dummy_sl_val ∗
-      is_uRPCClient cl_ptr host ∗
-      □(spec.(spec_Pre) x reqData)
+      "Hslice" ∷ own_slice_small req byteT 1 reqData ∗
+      "Hrep_out_ptr" ∷ rep_out_ptr ↦[slice.T byteT] dummy_sl_val ∗
+      "#Hclient" ∷ is_uRPCClient cl_ptr host ∗
+      "#Hhandler" ∷ is_urpc_spec γsmap host rpcid spec ∗
+      "#Hspec" ∷ □(spec.(spec_Pre) x reqData)
   }}}
     urpc.Client__Call #cl_ptr #rpcid (slice_val req) #rep_out_ptr #timeout_ms
   {{{
@@ -207,12 +157,41 @@ Lemma wp_Client__Call_uRPCSpec γsmap (cl_ptr:loc) (rpcid:u64) (host:u64) req re
           (spec.(spec_Post) x reqData repData))
   }}}.
 Proof.
-  iIntros (->) "#Hhandler !# %Φ Hpre HΦ".
-  iDestruct "Hpre" as "(Hslice&Hrep_out_ptr&Hclient&#HSpec)".
-  iApply (wp_Client__Call with "Hhandler [$Hrep_out_ptr $Hclient $Hslice]").
-  { simpl. do 2 iModIntro.
-    iExists _. iFrame "HSpec". iIntros (?) "Hpost". iExact "Hpost". }
+  iIntros (Φ) "Hpre HΦ".
+  iNamed "Hpre".
+  iApply (wp_Client__Call_pred with "[Hhandler Hrep_out_ptr Hclient Hslice]").
+  { iFrame "∗#".
+    simpl. do 2 iModIntro.
+    iExists _. iFrame "#". iIntros (?) "Hpost". iExact "Hpost". }
   done.
 Qed.
 
+Lemma wp_StartServer γ (host : u64) (handlers : gmap u64 val) (s : loc) :
+  dom handlers ≠ ∅ →
+  {{{
+      handlers_complete γ handlers ∗
+      own_Server s handlers ∗
+      [∗ map] rpcid ↦ handler ∈ handlers,
+      (∃ spec, is_urpc_spec γ host rpcid spec ∗ is_urpc_handler handler spec)
+  }}}
+    urpc.Server__Serve #s #host
+  {{{
+      RET #(); True
+  }}}.
+Proof.
+  iIntros (? Φ) "(#Hcomplete&Hserver&#His_rpc_map) HΦ".
+  wp_apply (wp_StartServer_pred with "[$Hserver]").
+  { done. }
+  { iFrame "#".
+    iApply (big_sepM_impl with "His_rpc_map").
+    iModIntro. iIntros (???) "[% [? ?]]".
+    iExists _. iFrame.
+    by iApply urpc_handler_to_handler.
+  }
+  by iApply "HΦ".
+Qed.
+
 End urpc_spec_impl.
+
+Arguments pnil {A}.
+Arguments pcons {A} a l.
