src/program_proof/memkv/memkv_coord_ghost_init.v
@@ -10,18 +10,18 @@ Section memkv_coord_ghost_init_proof.
 (* These lemmas happen *before* we get node local names (e.g. the gname for memory, crashes etc. *)
 Context `{!gooseGlobalGS Σ, erpcG Σ, urpcregG Σ, kvMapG Σ}.
 
-Definition coord_SpecList γkv : uRPCSpecList :=
-  spec_cons (is_coord_server_addSpec γkv)
-    (spec_cons (is_coord_server_getSpec γkv) spec_nil).
+Definition coord_SpecList γkv : plist (u64 * RpcSpec) :=
+  pcons (U64 uCOORD_ADD, is_coord_server_addSpec γkv)
+    (pcons (U64 uCOORD_GET, is_coord_server_getSpec γkv) pnil).
 
 Lemma coord_server_ghost_init host (γkv : gname) :
   host c↦ ∅ ={⊤}=∗
   ∃ γ, ⌜ γ.(coord_kv_gn) = γkv ⌝ ∗
-       is_urpc_dom γ.(coord_urpc_gn) (dom_uRPCSpecList (coord_SpecList (γ.(coord_kv_gn)))) ∗
+       is_urpc_dom γ.(coord_urpc_gn) (dom_RpcSpec_list (coord_SpecList (γ.(coord_kv_gn)))) ∗
        is_coord_server host γ.
 Proof.
   iIntros "Hg".
-  iMod (handler_is_init_list host (coord_SpecList γkv) with "[Hg]") as (γ) "H".
+  iMod (alloc_is_urpc_list host (coord_SpecList γkv) with "[Hg]") as (γ) "H".
   { simpl. set_solver. }
   { iExactEq "Hg". f_equal. }
   iDestruct "H" as "(#Hdom&#Hadd&#Hget&_)".
